formalize Stefan's idea

FSB.v
@@ -64,3 +64,34 @@ Proof.
 Qed.
 
 End Quick.
+
+
+Section Stefan.
+
+  Definition question_mark := forall P1 P2 Ct,
+    beh (Ct [P1 ↓]) ⊆ beh (Ct [P2 ↓]) -> 
+    exists Cs, beh (Cs [P1 ]) ⊆ beh (Cs [P2 ]).
+
+  Variable Wt : trace -> par src.
+ 
+  Hypothesis only_t:  forall Ct t t', sem tgt (Ct [(Wt t)↓]) t' -> t = t'. 
+  Hypothesis t_src : forall Cs t, sem src (Cs [(Wt t)]) t. (* CC for Wt *)  
+  
+  Lemma question_mark_RTC : question_mark -> RTC.
+  Proof.
+    rewrite RTC'. intros Hqm P Ct t Ht. 
+    destruct (classic (valid_trace P t)).
+    - exact H.
+    - unfold valid_trace in H. rewrite not_ex_forall_not in H.
+      destruct (Hqm (Wt t) P Ct) as [Cs HCs].
+      + intros b Hb. apply only_t in Hb. rewrite <- Hb. auto.
+      + exfalso. apply ((H Cs)). apply HCs. apply t_src.
+  Qed.       
+
+  (* CA: 
+     
+     only_t + t_src => ((~ valid P t) -> False)
+
+  *)
+  
+End Stefan. 
